examples/Employee_Model/Design_deep.thy
@@ -55,7 +55,7 @@ generation_syntax [ deep
                       (IMPORTS ["../src/UML_Main", "../src/compiler/OCL_compiler_static"]
                                "../src/compiler/OCL_compiler_generator_dynamic")
                       SECTION
-                      (*SORRY*)
+                      (*SORRY*) (*NO_DIRTY*)
                       [ (* in Haskell *)
                         (* in OCaml module_name M (no_signatures) *)
                         (* in Scala module_name M *)
