src/compiler/OCL_compiler_core.thy
@@ -344,7 +344,7 @@ definition "thy_ctxt_inv n = [ case n of Floor1 \<Rightarrow> OCL_compiler_floor
                                        | Floor2 \<Rightarrow> OCL_compiler_floor2_ctxt.print_ctxt_inv ]"
 definition "thy_flush_all = []"
 
-definition "ocl_compiler_config_empty disable_thy_output file_out_path_dep oid_start design_analysis sorry_mode =
+definition "ocl_compiler_config_empty disable_thy_output file_out_path_dep oid_start design_analysis sorry_dirty =
   ocl_compiler_config.make
     disable_thy_output
     file_out_path_dep
@@ -352,7 +352,7 @@ definition "ocl_compiler_config_empty disable_thy_output file_out_path_dep oid_s
     (0, 0)
     design_analysis
     None [] [] [] False False ([], []) []
-    sorry_mode"
+    sorry_dirty"
 
 definition "ocl_compiler_config_reset_no_env ocl =
   ocl_compiler_config_empty
@@ -360,7 +360,7 @@ definition "ocl_compiler_config_reset_no_env ocl =
     (D_file_out_path_dep ocl)
     (oidReinitAll (D_oid_start ocl))
     (D_design_analysis ocl)
-    (D_sorry_mode ocl)
+    (D_sorry_dirty ocl)
     \<lparr> D_ocl_env := D_ocl_env ocl \<rparr>"
 
 definition "ocl_compiler_config_reset_all ocl =
@@ -374,9 +374,9 @@ definition "ocl_compiler_config_reset_all ocl =
 
 definition "fold_thy0 univ thy_object0 f =
   List.fold (\<lambda>x (acc1, acc2).
-    let sorry_mode = D_sorry_mode acc1
+    let (sorry, dirty) = D_sorry_dirty acc1
       ; (l, acc1) = x univ acc1 in
-    (f (if sorry_mode then
+    (f (if sorry = Some Gen_sorry | sorry = None & dirty then
           List_map (hol_map_thy (hol_map_lemma (\<lambda> Lemma_by n spec _ _ \<Rightarrow> Lemma_by n spec [] Tacl_sorry
                                                 | Lemma_by_assum n spec1 spec2 _ _ \<Rightarrow> Lemma_by_assum n spec1 spec2 [] Tacl_sorry))) l
         else
